code/ecdsa/Hacl.Impl.EC.Masking.fst
@@ -1,0 +1,112 @@
+module Hacl.Impl.EC.Masking
+
+open FStar.HyperStack.All
+open FStar.HyperStack
+module ST = FStar.HyperStack.ST
+
+open Lib.IntTypes
+open Lib.Buffer
+
+open Hacl.Spec.P256.Definition
+open Lib.Loops
+
+open Spec.P256
+open Hacl.Lemmas.P256
+
+
+val copy_conditional: #c: curve 
+  -> out: felem c
+  -> x: felem c
+  -> mask: uint64{uint_v mask = 0 \/ uint_v mask = pow2 64 - 1} -> Stack unit 
+  (requires fun h -> live h out /\ live h x)
+  (ensures fun h0 _ h1 -> modifies (loc out) h0 h1 /\ (
+    if uint_v mask = 0 then as_nat c h1 out == as_nat c h0 out else as_nat c h1 out == as_nat c h0 x)
+  ) 
+
+
+let copy_conditional #c out x mask = 
+(*    let h0 = ST.get() in 
+  let out_0 = index out (size 0) in 
+  let out_1 = index out (size 1) in 
+  let out_2 = index out (size 2) in 
+  let out_3 = index out (size 3) in 
+
+  let x_0 = index x (size 0) in 
+  let x_1 = index x (size 1) in 
+  let x_2 = index x (size 2) in 
+  let x_3 = index x (size 3) in 
+
+  let r_0 = logxor out_0 (logand mask (logxor out_0 x_0)) in 
+  let r_1 = logxor out_1 (logand mask (logxor out_1 x_1)) in 
+  let r_2 = logxor out_2 (logand mask (logxor out_2 x_2)) in 
+  let r_3 = logxor out_3 (logand mask (logxor out_3 x_3)) in 
+
+
+  lemma_xor_copy_cond out_0 x_0 mask;
+  lemma_xor_copy_cond out_1 x_1 mask;
+  lemma_xor_copy_cond out_2 x_2 mask;
+  lemma_xor_copy_cond out_3 x_3 mask;
+
+ 
+  upd out (size 0) r_0;
+  upd out (size 1) r_1;
+  upd out (size 2) r_2;
+  upd out (size 3) r_3;
+    let h1 = ST.get() in 
+
+  lemma_eq_funct_ (as_seq h1 out) (as_seq h0 out);
+  lemma_eq_funct_ (as_seq h1 out) (as_seq h0 x)
+*)
+  let h0 = ST.get() in
+  
+  let len = getCoordinateLenU64 c in 
+  let inv h (i: nat { i <= uint_v (getCoordinateLenU64 c)}) = True in 
+  for 0ul len inv (fun i -> 
+    let h_ = ST.get() in 
+    let x_i = index x i in 
+    let out_i = index out i in 
+    let r_i = logxor out_i (logand mask (logxor out_i x_i)) in 
+    upd out i r_i
+  )
+
+  
+
+
+val cmovznz4: #c: curve -> cin: uint64 -> x: felem c -> y: felem c -> result: felem c ->
+  Stack unit
+  (requires fun h -> live h x /\ live h y /\ live h result /\ disjoint x result /\ eq_or_disjoint y result)
+  (ensures fun h0 _ h1 -> modifies1 result h0 h1 /\ (
+    if uint_v cin = 0 then as_nat c h1 result == as_nat c h0 x 
+    else as_nat c h1 result == as_nat c h0 y)
+  )
+
+let cmovznz4 #c  cin x y r =
+  let h0 = ST.get() in
+  let mask = neq_mask cin (u64 0) in
+  
+  let len = getCoordinateLenU64 c in 
+  let inv h (i: nat { i <= uint_v (getCoordinateLenU64 c)}) = 
+    live h x /\ live h y /\ modifies (loc r) h0 h /\ 
+    (
+      forall (j: nat {j >= i && j < v (getCoordinateLenU64 c)}).
+      let y_i = Lib.Sequence.index (as_seq h y) j in 
+      let y_0 = Lib.Sequence.index (as_seq h0 y) j in 
+      uint_v y_i == uint_v y_0
+    ) /\ (
+      forall (j: nat {j < i}).
+	let x_i = Lib.Sequence.index (as_seq h0 x) j in 
+	let y_i = Lib.Sequence.index (as_seq h0 y) j in 
+	let r_i = Lib.Sequence.index (as_seq h r) j in 
+	if uint_v cin = 0 then 
+	  uint_v r_i == uint_v x_i
+	else
+	  uint_v r_i == uint_v y_i
+    ) in 
+  for 0ul len inv (fun i -> 
+    let h_ = ST.get() in 
+    let x_i = index x i in 
+    let y_i = index y i in 
+    let r_i = logor (logand y_i mask) (logand x_i (lognot mask)) in 
+    upd r i r_i;
+    cmovznz4_lemma cin (Seq.index (as_seq h0 x) (v i)) (Seq.index (as_seq h0 y) (v i))
+  )
